backend/RTLC.v
@@ -12,11 +12,13 @@ Set Implicit Arguments.
 
 Local Obligation Tactic := ii; ss; des; inv_all_once; ss; clarify.
 
+Definition fn_ssig := fun fd => Some (fd.(fn_sig)).
+
 Section MODSEM.
 
   Variable skenv_link: SkEnv.t.
   Variable p: program.
-  Let skenv: SkEnv.t := skenv_link.(SkEnv.project) p.(Sk.of_program (Some <*> fn_sig)).
+  Let skenv: SkEnv.t := skenv_link.(SkEnv.project) p.(Sk.of_program fn_ssig).
   Let ge: genv := skenv.(SkEnv.revive) p.
 
   Inductive at_external: state -> Args.t -> Prop :=
@@ -112,7 +114,7 @@ Section MODSEM.
 End MODSEM.
 
 Program Definition module (p: program): Mod.t :=
-  {| Mod.data := p; Mod.get_sk := Sk.of_program (Some <*> fn_sig); Mod.get_modsem := modsem; |}.
+  {| Mod.data := p; Mod.get_sk := Sk.of_program fn_ssig; Mod.get_modsem := modsem; |}.
 
 Program Definition module2 (p: program): Mod.t :=
-  {| Mod.data := p; Mod.get_sk := Sk.of_program (Some <*> fn_sig); Mod.get_modsem := modsem2; |}.
+  {| Mod.data := p; Mod.get_sk := Sk.of_program fn_ssig; Mod.get_modsem := modsem2; |}.
