backend/ValueAnalysisC.v
@@ -16,7 +16,7 @@ Require Import ModSem.
 
 Lemma sound_state_sound_args
       bc m0 stack su0 p skenv_link vs_arg cunit ge
-      (GENV: ge = (SkEnv.revive (SkEnv.project skenv_link p.(Sk.of_program fn_sig)) p))
+      (GENV: ge = (SkEnv.revive (SkEnv.project skenv_link p.(Sk.of_program fn_ssig)) p))
       (STK: sound_stack cunit ge su0 bc stack m0 (Mem.nextblock m0))
       (ARGS: forall v : val, In v vs_arg -> vmatch bc v Vtop)
       (RO: romatch bc m0 (romem_for cunit))
@@ -24,7 +24,7 @@ Lemma sound_state_sound_args
       (GE: genv_match bc ge)
       (NOSTK: bc_nostack bc)
       fptr_arg sg_arg
-      (SIG: exists skd, Genv.find_funct skenv_link fptr_arg = Some skd /\ SkEnv.get_sig skd = sg_arg):
+      (SIG: exists skd, Genv.find_funct skenv_link fptr_arg = Some skd /\ Sk.get_sig skd = sg_arg):
     args' (bc2su bc ge.(Genv.genv_next) m0.(Mem.nextblock)) (Args.mk fptr_arg vs_arg m0).
 Proof.
   { r. s. esplits; eauto.
@@ -74,7 +74,7 @@ Qed.
 (* copied from above *)
 Lemma sound_state_sound_retv
       bc m_ret su0 p skenv_link v_ret cunit ge
-      (GENV: ge = (SkEnv.revive (SkEnv.project skenv_link p.(Sk.of_program fn_sig)) p))
+      (GENV: ge = (SkEnv.revive (SkEnv.project skenv_link p.(Sk.of_program fn_ssig)) p))
       (STK: sound_stack cunit ge su0 bc [] m_ret (Mem.nextblock m_ret))
       (RES: vmatch bc v_ret Vtop)
       (RO: romatch bc m_ret (romem_for cunit))
@@ -131,7 +131,7 @@ Section PRSV.
   Variable skenv_link: SkEnv.t.
   Variable p: program.
 
-  Hypothesis INCL: SkEnv.includes skenv_link (Sk.of_program fn_sig p).
+  Hypothesis INCL: SkEnv.includes skenv_link (Sk.of_program fn_ssig p).
 
   Let modsem := RTLC.modsem skenv_link p.
 
@@ -143,9 +143,9 @@ Section PRSV.
     econs; eauto.
     { ss. eapply UnreachC.liftspec; et. }
     - i. inv INIT. ss. esplits; eauto; cycle 1.
-      { refl. }
+      { destruct args; ss. refl. }
       econs; eauto. i.
-      set (ge := (SkEnv.revive (SkEnv.project skenv_link p.(Sk.of_program fn_sig)) p)) in *.
+      set (ge := (SkEnv.revive (SkEnv.project skenv_link p.(Sk.of_program fn_ssig)) p)) in *.
       set (f := fun b =>
                   if plt b (Genv.genv_next ge) then
                     match Genv.invert_symbol ge b with None => BCglob None | Some id => BCglob (Some id) end
@@ -158,11 +158,13 @@ Section PRSV.
         - ii. subst f. ss. des_ifs. apply_all_once Genv.invert_find_symbol. clarify.
       }
       subst f. des.
-      r in SUARG. des. ss. unfold Sound.vals in *. rewrite Forall_forall in *.
+      assert(T: <<VAL: val' su_init (Args.fptr args)>> /\ <<VALS: Sound.vals su_init (Args.vs args)>> /\ <<MEM: mem' su_init (Args.m args)>> /\ <<WF: Unreach.wf su_init>>).
+      { r in SUARG. des_ifs. }
+      clear SUARG. des. ss. unfold Sound.vals in *. rewrite Forall_forall in *.
       assert(FP: forall blk, su_init blk -> Ple ge.(Genv.genv_next) blk).
       { inv SKENV. ss. i. inv MEM. rewrite <- PUB. apply NNPP. ii. inv WF. exploit WFHI; eauto. }
       assert(NB: Ple ge.(Genv.genv_next) args.(Args.m).(Mem.nextblock)).
-      { inv SKENV. ss. }
+      { inv SKENV. ss. destruct args; ss. }
       assert(GE: genv_match bc ge).
       { r. esplits; eauto.
         * ii. rewrite IMG in *. split; i.
@@ -186,7 +188,7 @@ Section PRSV.
         { eapply nth_error_In; eauto. }
         repeat spc VALS. specialize (VALS eq_refl). (* TODO: fix spc ... *) des.
         des_ifs; ss. bsimpl. des; ss. des_sumbool. inv MEM. congruence.
-      + inv SKENV. ss. clear - IMG ROMATCH H INCL.
+      + inv SKENV. ss. clear - IMG ROMATCH H INCL CSTYLE.
         ii. exploit (ROMATCH b id ab); eauto.
         { rewrite IMG in *. des_ifs. ss. des_ifs.
           - clear - Heq Heq0. eapply Genv.invert_find_symbol in Heq. subst ge. unfold SkEnv.revive in *.
@@ -202,12 +204,12 @@ Section PRSV.
           exploit SkEnv.project_impl_spec; et. intro PROJ.
           exploit SkEnv.project_revive_precise; et. intro PRECISE. inv PRECISE.
           exploit P2GE; et. i; des. ss. unfold fundef in *. folder. clarify.
-          assert(INTSID: internals (Sk.of_program fn_sig p) id).
+          assert(INTSID: internals (Sk.of_program fn_ssig p) id).
           { rewrite Sk.of_program_internals. unfold internals. des_ifs. }
-          assert(DEFSID: defs (Sk.of_program fn_sig p) id).
+          assert(DEFSID: defs (Sk.of_program fn_ssig p) id).
           { eapply internals_defs; et. }
           assert(BIG: Genv.find_def skenv_link b = Some (Gvar v)).
-          { generalize (Sk.of_program_prog_defmap p fn_sig id). intro REL.
+          { generalize (Sk.of_program_prog_defmap p fn_ssig id). intro REL.
             inv REL; try congruence. rewrite LOA in *. clarify.
             assert(y = Gvar v).
             { inv H1. inv H2. ss. destruct i1, i2; ss. }
@@ -222,14 +224,14 @@ Section PRSV.
             inv MATCH. inv H0. destruct info1, info2; ss.
             inv H1; ss.
           }
-          assert(SMALL: Genv.find_def (SkEnv.project skenv_link (Sk.of_program fn_sig p)) b = Some (Gvar v)).
+          assert(SMALL: Genv.find_def (SkEnv.project skenv_link (Sk.of_program fn_ssig p)) b = Some (Gvar v)).
           { inv PROJ.
             exploit DEFKEEP; et.
             { apply Genv.find_invert_symbol; et. rewrite <- SYMBKEEP; et. }
             i; des.
             assert(gd_small = (Gvar v)).
             { (* TODO: make lemma!!!!!!!!!!!!!!!!! *)
-              clear - PROG LOA. generalize (Sk.of_program_prog_defmap p fn_sig id). intro REL.
+              clear - PROG LOA. generalize (Sk.of_program_prog_defmap p fn_ssig id). intro REL.
               inv REL; try congruence.
               rewrite LOA in *. rewrite PROG in *. clarify.
               inv H1. inv H0. repeat f_equal. destruct i1, i2; ss.
@@ -238,6 +240,7 @@ Section PRSV.
           }
           unfold Genv.find_var_info. des_ifs.
         }
+        rewrite Args.get_m_m in *; ss. 
         intro RO; des. esplits; et. eapply bmatch_incr; et.
         ii. ss. rewrite IMG. des_ifs.
         * clear - Heq Heq0. eapply Genv.invert_find_symbol in Heq. subst ge. unfold SkEnv.revive in *.
@@ -300,26 +303,27 @@ Section PRSV.
         inv AT. inv H; ss.
         exploit sound_state_sound_args; eauto. i.
         hexploit (@UnreachC.greatest_ex (bc2su bc (Genv.genv_next skenv_link) (Mem.nextblock m0)) args0); eauto.
-        { esplits; eauto. ss. refl. }
+        { subst args0. r in H. des. esplits; eauto; cycle 1. { r. ss. esplits; eauto. } ss. refl. }
         i; des. ss. esplits; eauto.
         - exploit (@UnreachC.get_greatest_le); ss; eauto.
+          { subst args0; ss. }
           + eapply UnreachC.hle_lift; eauto.
         - rr in GR. des. etrans; eauto. eapply UnreachC.hle_lift; eauto.
       }
       des. esplits; eauto.
       { inv AT; ss. refl. }
       { exploit H; eauto. { apply linkorder_refl. } intro T; des. inv T; ss. }
-      { eapply GR; eauto. }
+      { r in GR. inv AT. ss. des. r in PROP0. des. esplits; et. }
       { refl. }
       ii. r in RETV. des. esplits; eauto; cycle 1.
-      { inv AT; inv AFTER; ss. refl. }
+      { inv AT; inv AFTER; ss. rewrite Retv.get_m_m; ss. refl. }
       + econs; eauto. intros cunit LO. specialize (H cunit LO). inv AFTER; ss. inv H; ss.
         assert(BCARGS: (bc2su bc (Genv.genv_next skenv_link) m_arg.(Mem.nextblock)).(Sound.args) args).
-        { ss. inv AT; ss. r. s. rpapply sound_state_sound_args; eauto. }
+        { ss. inv AT; ss. s. rpapply sound_state_sound_args; eauto. }
         assert(BCLE0: le' su0 (bc2su bc (Genv.genv_next skenv_link) m_arg.(Mem.nextblock))).
         { eapply UnreachC.hle_lift; eauto. }
         assert(BCLE1: le' (bc2su bc (Genv.genv_next skenv_link) m_arg.(Mem.nextblock)) su_gr).
-        { eapply GR; eauto. }
+        { eapply GR; eauto. esplits; eauto. inv AT. ss. }
         set (f := fun b => if plt b (Mem.nextblock m_arg)
                            then bc b
                            else
@@ -339,23 +343,23 @@ Section PRSV.
                                      (bc2su bc' (Genv.genv_next skenv_link) (Mem.nextblock (Retv.m retv)))).
         { rr. ss. rewrite IMG. unfold f.
           assert(NB: Ple (Mem.nextblock m_arg) (Mem.nextblock (Retv.m retv))).
-          { inv AT; ss. inv MLE. inv RO0. ss. }
+          { inv AT; ss. rewrite Retv.get_m_m in *; ss. inv MLE. inv RO0. ss. }
           esplits; ss.
           - i. des_ifs. xomega.
         }
 
         assert(GRARGS: Sound.args su_gr args).
-        { rr in GR. des. ss. }
+        { rr in GR. des. inv AT; ss. }
         exploit Unreach.hle_hle_old; try apply LE; eauto.
-        { rr in GRARGS. des. ss. }
+        { rr in GRARGS. des. inv AT; ss. des; ss. }
         intro LEOLD.
         assert (VMTOP0: forall v, Sound.val su_gr v -> vmatch bc' v Vtop).
         { i. ss. r in H. destruct v; econs; eauto. econs; eauto.
           exploit H; eauto. i; des. rewrite IMG. subst f. s. des_ifs_safe.
           assert(NBC: ~ (bc2su bc (Genv.genv_next skenv_link) m_arg.(Mem.nextblock)) b).
           { ii. ss. r in BCLE1. des. exploit PRIV; eauto. des_ifs. }
-          ss. inv MEM. rr in GRARGS. des. inv MEM. ss.
-          inv AT; ss. rewrite NB0 in *. des_ifs; try xomega.
+          ss. des. inv MEM. rr in GRARGS. inv AT; ss. des. inv MEM. ss.
+          rewrite NB0 in *. des_ifs; try xomega.
           intro BC. unfold bc2su in *. ss. rewrite BC in *. ss.
         }
         assert (VMTOP: forall v, val' su_ret v -> vmatch bc' v Vtop).
@@ -365,7 +369,7 @@ Section PRSV.
           { ii. r in LEOLD. des. exploit PRIV; eauto. i; ss. congruence. }
           assert(NBC: ~ (bc2su bc (Genv.genv_next skenv_link) m_arg.(Mem.nextblock)) b).
           { ii. ss. r in BCLE1. des. exploit PRIV; eauto. des_ifs. }
-          ss. inv MEM. rewrite NB in *. des_ifs.
+          ss. des. inv MEM. rewrite NB in *. des_ifs.
           clear - NBC p0.
           ii. unfold bc2su in *. ss. rewrite H in *. ss.
         }
@@ -396,8 +400,8 @@ Section PRSV.
         { intros; split; intros.
           - destruct (su_gr b) eqn:T.
             + assert(Plt b (Mem.nextblock m_arg)).
-              { rr in GRARGS. des. inv MEM0. inv AT; ss.
-                inv WF1. exploit WFHI; eauto. i. Unreach.nb_tac. ss.
+              { rr in GRARGS. inv AT; ss. des. inv MEM.
+                inv WF0. exploit WFHI; try apply T. eauto. i. Unreach.nb_tac. ss.
               }
               rewrite IMG in *. subst f. ss. des_ifs.
 
@@ -409,13 +413,13 @@ Section PRSV.
               { rewrite IMG in *. subst f. ss. des_ifs.
                 rr in LE. des. ss. erewrite <- OLD; eauto.
                 { congruence. }
-                rr in GRARGS. des. inv MEM0. inv AT; ss. Unreach.nb_tac. ss.
+                rr in GRARGS. inv AT; ss. des. inv MEM0. Unreach.nb_tac. ss.
               }
-              eapply VMTOP; eauto. eapply mem'_load_val'; eauto.
+              eapply VMTOP; eauto. eapply mem'_load_val'; eauto. inv AT; ss. des_ifs; des; ss.
           - destruct (su_gr b) eqn:T.
             + assert(Plt b (Mem.nextblock m_arg)).
-              { rr in GRARGS. des. inv MEM0. inv AT; ss.
-                inv WF1. exploit WFHI; eauto. i.
+              { rr in GRARGS. inv AT; ss. des. inv MEM.
+                inv WF0. exploit WFHI; eauto. i.
                 Unreach.nb_tac. ss.
               }
               rewrite IMG in *. subst f. ss. des_ifs.
@@ -428,10 +432,10 @@ Section PRSV.
               assert(~ su_ret b).
               { rewrite IMG in *. subst f. ss. des_ifs.
                 rr in LE. des. ss. erewrite <- OLD; eauto; try congruence.
-                rr in GRARGS. des. inv MEM0. inv AT; ss. Unreach.nb_tac. ss.
+                rr in GRARGS. des. inv AT; ss. des. inv MEM0. Unreach.nb_tac. ss.
               }
               eapply PMTOP; eauto; cycle 1.
-              { inv MEM.
+              { inv AT; ss. des_ifs; des. inv MEM1.
                 Local Transparent Mem.loadbytes.
                 unfold Mem.loadbytes in *. des_ifs.
                 exploit (SOUND b ofs); eauto.
@@ -439,8 +443,10 @@ Section PRSV.
                 i; des. ss. Unreach.nb_tac. xomega.
               }
               eapply mem'_loadbytes_val'; eauto.
+              des_ifs; des; ss.
         }
 
+        rewrite Retv.get_m_m in *; ss.
         eapply sound_return_state with (bc := bc'); eauto.
         * apply sound_stack_new_bound with (Mem.nextblock m_arg); cycle 1.
           { inv HLEAFTER. des. ss. }
@@ -450,7 +456,7 @@ Section PRSV.
           i. inv MLE. inv AT. ss.
           eapply Mem.loadbytes_unchanged_on_1; try apply PRIV; eauto.
           u. i. eapply BCLE1; et. ss. des_ifs. des_sumbool. ss.
-        * eapply VMTOP; et. unfold typify. des_ifs.
+        * eapply VMTOP; et. unfold typify. des_ifs. des; ss.
         * eapply romatch_exten; cycle 1.
           { instantiate (1 := bc). rewrite IMG. subst f. split; i; try by des_ifs.
             des_ifs_safe. exfalso. eapply n. eapply mmatch_below. eauto. congruence.
@@ -472,7 +478,7 @@ Section PRSV.
                 exploit Genv.find_invert_symbol; et. intro INV. rewrite INV. ss.
               + eapply romem_for_ske_complete; et. clear - LO X INCL Y0 X2. inv INCL.
                 exploit (prog_defmap_linkorder cunit); et. intro Z; des.
-                hexploit (Sk.of_program_prog_defmap p fn_sig id); et. intro REL.
+                hexploit (Sk.of_program_prog_defmap p fn_ssig id); et. intro REL.
                 unfold fundef in *. rewrite Z in REL. inv REL. symmetry in H0.
                 exploit DEFS; et. intro W; des.
                 assert(b = blk).
@@ -512,8 +518,8 @@ Section PRSV.
     - ii. inv FINAL. s.
       inv SUST. specialize (H p (linkorder_refl _)). inv H.
       exists (bc2su bc (Genv.genv_next skenv_link) m_ret.(Mem.nextblock)).
+      exploit sound_state_sound_retv; try apply STK; eauto; ss. i; des.
       esplits; try refl; ss; eauto.
-      rp; [eapply sound_state_sound_retv; eauto|..]; eauto.
   Qed.
 
 End PRSV.
